src/Semantics/InterpStateIneq.dfy
@@ -1,0 +1,270 @@
+include "../Interop/CSharpDafnyASTModel.dfy"
+include "../Interop/CSharpInterop.dfy"
+include "../Interop/CSharpDafnyInterop.dfy"
+include "../Interop/CSharpDafnyASTInterop.dfy"
+include "../Utils/Library.dfy"
+include "../Utils/StrTree.dfy"
+include "Interp.dfy"
+include "Equiv.dfy"
+include "ExprInduction.dfy"
+
+module Bootstrap.Semantics.InterpStateIneq {
+  // This module provides lemmas which prove that the environment is monotonous (the set of
+  // variables grows).
+
+module Base refines ExprInduction.Ind {
+  //
+  // Declarations
+  //
+  type Value = Interp.Value
+
+  datatype MState = MState(env: Environment, ctx: State)
+
+  type S(!new) = MState
+  type V(!new) = Value
+  type VS(!new) = seq<Value>
+
+  predicate StateSmaller(ctx: State, ctx': State)
+  {
+    // We have to pay attention to one thing, which is that when we evaluate a variable declaration,
+    // we *remove* the binding from the local variables, but if this binding is already present,
+    // we save it in the rollback.
+    ctx.locals.Keys + ctx.rollback.Keys <= ctx'.locals.Keys + ctx'.rollback.Keys
+  }
+
+  predicate InterpResultStateSmaller<V>(ctx: State, res: InterpResult<V>)
+  {
+    match res
+      case Success(Return(_, ctx')) => StateSmaller(ctx, ctx')
+      case Failure(_) => true
+  }
+
+  predicate P(st: S, e: Expr)
+  {
+    InterpResultStateSmaller(st.ctx, InterpExpr(e, st.env, st.ctx))
+  }
+  
+  predicate P_Succ(st: S, e: Expr, st': S, v: V)
+  {
+    && InterpResultStateSmaller(st.ctx, InterpExpr(e, st.env, st.ctx))
+    && InterpExpr(e, st.env, st.ctx) == Success(Return(v, st'.ctx))
+    && st.env == st'.env
+  }
+
+  predicate P_Fail(st: S, e: Expr)
+  {
+    InterpExpr(e, st.env, st.ctx).Failure?
+  }
+
+  predicate Pes(st: S, es: seq<Expr>)
+  {
+    InterpResultStateSmaller(st.ctx, InterpExprs(es, st.env, st.ctx))
+  }
+
+  predicate Pes_Succ(st: S, es: seq<Expr>, st': S, vs: VS)
+  {
+    && InterpResultStateSmaller(st.ctx, InterpExprs(es, st.env, st.ctx))
+    && InterpExprs(es, st.env, st.ctx) == Success(Return(vs, st'.ctx))
+    && st.env == st'.env
+  }
+
+  predicate Pes_Fail(st: S, es: seq<Expr>)
+  {
+    InterpExprs(es, st.env, st.ctx).Failure?
+  }
+
+  function AppendValue ...
+  {
+    [v] + vs
+  }
+
+  function SeqVToVS ...
+  {
+    vs
+  }
+  
+  function GetNilVS ...
+  {
+    []
+  }
+
+  ghost const UnitV := Values.Unit
+
+  function VS_Last ...
+  {
+    vs[|vs| - 1]
+  }
+
+  predicate VS_UpdateStatePre ...
+  {
+    && |argvs| == |vars|
+  }
+
+  function BuildClosureCallState ...
+  {
+    var ctx1 := BuildCallState(st.ctx.locals, vars, argvs);
+    MState(st.env, ctx1)
+  }
+
+  function UpdateState ...
+  {
+    var ctx1 := st.ctx.(locals := AugmentContext(st.ctx.locals, vars, vals));
+    MState(st.env, ctx1)
+  }
+
+  function StateSaveToRollback ...
+  {
+    var ctx := SaveToRollback(st.ctx, vars);
+    var st' := MState(st.env, ctx);
+    st'
+  }
+
+  function StateStartScope ...
+  {
+    var ctx := StartScope(st.ctx);
+    MState(st.env, ctx)
+  }
+
+  function StateEndScope ...
+  {
+    var ctx := EndScope(st0.ctx, st.ctx);
+    MState(st.env, ctx)
+  }
+
+  function P_Step ... {
+    var Return(v, ctx1) := InterpExpr(e, st.env, st.ctx).value;
+    (MState(st.env, ctx1), v)
+  }
+
+  function Pes_Step ... {
+    var Return(vs, ctx1) := InterpExprs(es, st.env, st.ctx).value;
+    (MState(st.env, ctx1), vs)
+  }
+
+  //
+  // Lemmas
+  //
+
+  lemma P_Fail_Sound ... {}
+  lemma P_Succ_Sound ... {}
+  lemma Pes_Fail_Sound ... {}
+  lemma Pes_Succ_Sound ... {}
+
+  lemma Pes_Succ_Inj ... {}
+  lemma SeqVToVS_Append ... {}
+
+  lemma InductVar ... { reveal InterpExpr(); }
+
+  lemma InductLiteral ... { reveal InterpExpr(); }
+
+  lemma InductAbs ... { reveal InterpExpr(); }
+
+  lemma InductAbs_CallState ... {
+    reveal InterpExpr();
+    reveal InterpCallFunctionBody();
+    reveal BuildCallState();
+  }
+
+  lemma InductExprs_Nil ... { reveal InterpExprs(); }
+  lemma InductExprs_Cons ... { reveal InterpExprs(); }
+
+  lemma InductApplyLazy_Fail ... { reveal InterpExpr(); reveal InterpLazy(); }
+  lemma InductApplyLazy_Succ ... { reveal InterpExpr(); reveal InterpLazy(); }
+
+  lemma InductApplyEager_Fail ... { reveal InterpExpr(); }
+
+  lemma InductApplyEagerUnaryOp_Succ ... { reveal InterpExpr(); }
+  lemma InductApplyEagerBinaryOp_Succ ... { reveal InterpExpr(); }
+  lemma InductApplyEagerTernaryOp_Succ ... { reveal InterpExpr(); }
+  lemma InductApplyEagerBuiltinDisplay ... { reveal InterpExpr(); }
+  lemma InductApplyEagerFunctionCall ... { reveal InterpExpr(); }
+
+  lemma InductIf_Fail ... { reveal InterpExpr(); }
+  lemma InductIf_Succ ... { reveal InterpExpr(); }
+
+  lemma InductUpdate_Fail ... { reveal InterpExpr(); }
+  lemma InductUpdate_Succ ... { reveal InterpExpr(); }
+
+  lemma InductVarDecl_None_Succ ... { reveal InterpExpr(); reveal SaveToRollback(); }
+  lemma InductVarDecl_Some_Fail ... { reveal InterpExpr(); }
+  lemma InductVarDecl_Some_Succ  ... { reveal InterpExpr(); reveal SaveToRollback(); }
+
+  // TODO(SMH): I tried simplifying the proofs below by adding a `requires` in ``InductBlock_Fail``
+  // and ``InductBlock_Succ`` to provide the assertions and the results of calling the lemmas used
+  // in the proof below, but it didn't work due to SMT solvers' misteries.
+  lemma InductBlock_Fail ...
+  {
+    reveal InterpExpr();
+    reveal InterpBlock();
+    reveal InterpExprs();
+    reveal InterpBlock_Exprs();
+    reveal InterpExprs_Block();
+
+    var env := st.env;
+
+    // We need this because of the fuel
+    assert InterpExpr(e, env, st.ctx) == InterpBlock(stmts, env, st.ctx);
+    
+    InterpExprs_Block_Equiv_Strong(stmts, env, st_start.ctx);
+  }
+
+  lemma InductBlock_Succ ...
+  {
+    reveal InterpExpr();
+    reveal InterpBlock();
+    reveal InterpExprs();
+    reveal InterpBlock_Exprs();
+    reveal InterpExprs_Block();
+
+    var env := st.env;
+
+    // We need this because of the fuel
+    assert InterpExpr(e, env, st.ctx) == InterpBlock(stmts, env, st.ctx);
+    
+    InterpExprs_Block_Equiv_Strong(stmts, env, st_start.ctx);
+  }
+
+} // end of module Bootstrap.Semantics.EqInterpRefl.Base
+
+  import opened AST.Syntax
+  import opened Utils.Lib
+  import opened AST.Predicates
+  import opened Interp
+  import opened Values
+  import opened Equiv
+  import opened Utils.Lib.Datatypes
+  import opened Base
+
+  type Expr = Interp.Expr
+  ghost const StateSmaller := Base.StateSmaller
+  predicate InterpResultStateSmaller<V>(ctx: State, res: InterpResult<V>)
+  {
+    Base.InterpResultStateSmaller(ctx, res)
+  }
+
+  lemma InterpBlock_Exprs_StateSmaller(es: seq<Expr>, env: Environment, ctx: State)
+    // TODO(SMH): for some reason, using ``Seq_All`` makes some proofs fail. The weird thing is
+    // that I can then prove `Seq_All(SupportsInterp, es)` in an assertion just before the call
+    // to the lemma, but the lemma precondition keeps failing.
+    requires forall e | e in es :: SupportsInterp(e)
+    ensures InterpResultStateSmaller(ctx, InterpBlock_Exprs(es, env, ctx))
+  {
+    InterpExprs_Block_Equiv_Strong(es, env, ctx);
+    Base.Pes_Satisfied(MState(env, ctx), es);
+
+    reveal InterpExprs_Block();
+  }
+
+  lemma InterpExprs_StateSmaller(es: seq<Expr>, env: Environment, ctx: State)
+    ensures InterpResultStateSmaller(ctx, InterpExprs(es, env, ctx))
+  {
+    Base.Pes_Satisfied(MState(env, ctx), es);
+  }
+
+  lemma InterpExpr_StateSmaller(e: Expr, env: Environment, ctx: State)
+    ensures InterpResultStateSmaller(ctx, InterpExpr(e, env, ctx))
+  {
+    Base.P_Satisfied(MState(env, ctx), e);
+  }
+
+} // end of module Bootstrap.Semantics.EqInterpRefl
